BoC/Common.lean
@@ -75,18 +75,6 @@ postfix:80 " * " => Relation.ReflTransGen
 
 
 -- Relation lemmas
-lemma TransGen_right_induction {α : Type*} {r : α → α → Prop} {P : α → α → Prop} :
-  (∀a b, r a b → P a b) →
-  (∀a b c, r a b → P b c → P a c) →
-  (∀a b, (r +) a b → P a b) :=
-  by
-    intro h_base h_step a b h_clos
-    induction h_clos with
-    | @single b' h_rel =>
-      exact h_base a b' h_rel
-    | @tail a' b' h_clos h_rel ih =>
-      sorry
-
 
 -- List lemmas
 lemma pair_infix_inv {A} {l : List A} {x1 x2} :
